compiler/src/RegAllocAnnotatedNotations.v
@@ -1,0 +1,24 @@
+Require Import bedrock2.Basic_bopnames.
+Require Import compiler.RegAlloc3.
+
+Export bopname.
+
+Notation "a ; b" := (ASSeq _ _ _ a b) (only printing, right associativity,
+      at level 50, format "a ; '//' b") : regalloc_scope.
+Notation "'$x' a '($r' b ')' = c" := (ASLit _ _ _ a b c) (only printing,
+      at level 40, format "'$x' a '($r' b ')'  =  c") : regalloc_scope.
+Notation "'$x' a '($r' b ')' = '$x' c" := (ASSet _ _ _ a b c) (only printing,
+      at level 40, format "'$x' a '($r' b ')'  =  '$x' c") : regalloc_scope.
+Notation "'$x' a '($r' b ')' = op '$x' c '$x' d" := (ASOp _ _ _ a b op c d) (only printing,
+      at level 40, format "'$x' a '($r' b ')'  =  op  '$x' c  '$x' d") : regalloc_scope.
+Notation "'loop' a 'breakUnless' '$x' cond b" := (ASLoop _ _ _ a cond b)
+      (only printing, at level 50, a at level 40,
+       format "'loop' '[v ' '//' a '//' 'breakUnless'  '$x' cond '//' b ']'") : regalloc_scope.
+Notation "'skip'" := (ASSkip _ _ _) (only printing) : regalloc_scope.
+
+(* TODO
+       ASLoad(x: srcvar)(x': impvar)(a: srcvar)
+       ASStore(a: srcvar)(v: srcvar)
+       ASIf(cond: srcvar)(bThen bElse: astmt)
+       ASSkip
+       ASCall(binds: list (srcvar * impvar))(f: func)(args: list srcvar). *)
