compiler/src/examples/CompileExamples.v
@@ -1,0 +1,115 @@
+Require Import Coq.Lists.List.
+Import ListNotations.
+Require Import Coq.Strings.String.
+Require bedrock2.Examples.Demos.
+Require Import bedrock2.Basic_bopnames.
+Require Import lib.LibTacticsMin.
+Require Import riscv.util.Word.
+Require Import compiler.Decidable.
+Require Import compiler.Op.
+Require Import compiler.ExprImp.
+Require Import compiler.NameGen.
+Require Import compiler.Pipeline.
+Require Import compiler.util.Common.
+Require Import riscv.ListMemory.
+Require Import riscv.util.BitWidths.
+Require Import riscv.util.BitWidth32.
+Require Import riscv.MachineWidth32.
+Require Import compiler.FlatToRiscv32Proofs.
+Require Import compiler.FlatToRiscv32Specifics.
+Require Import compiler.util.List_Map.
+Require Import compiler.ZNameGen.
+Require Import riscv.InstructionCoercions.
+Require compiler.FlatImp.
+Require Import compiler.RegAlloc3.
+Require Import bedrock2.Byte.
+Require Import compiler.RegAllocAnnotatedNotations.
+Require Import riscv.InstructionNotations.
+Require Import bedrock2.Hexdump.
+
+Open Scope Z_scope.
+Open Scope string_scope.
+Open Scope regalloc_scope.
+
+Definition var: Set := Z.
+Definition func: Set := Empty_set.
+Definition Reg: Set := Z.
+
+Existing Instance MachineWidth32.MachineWidth32.
+
+Existing Instance DefaultRiscvState.
+
+Existing Instance FlatToRiscv.State_is_RegisterFile.
+
+Record example := mk_example {
+  name: string;
+  inputVars: set var;
+  outputVars: set var;
+  src: cmd;
+  flattened: FlatImp.stmt var func;
+  regallocAnnotated: astmt var var func;
+  regallocChecked: FlatImp.stmt var func;
+  riscv_instructions: list Instruction;
+  riscv_bytes: list byte;
+}.
+
+Arguments mk_example
+          name%string
+          inputVars
+          outputVars
+          src
+          flattened
+          regallocAnnotated%regalloc_scope
+          regallocChecked
+          riscv_instructions (* TODO add scope to riscv.InstructionNotations *)
+          riscv_bytes%hexdump_scope.
+
+Instance bops: @BasicALU.operations (@syntax Basic32Semantics.Basic32Semantics) :=
+  @Basic_bopnames.BasicALU {|
+    Basic_bopnames.varname := var;
+    Basic_bopnames.funcname := func;
+    Basic_bopnames.actname := Empty_set;
+  |}.
+
+Definition list_to_id_map(l: list var): map var var :=
+  fold_left (fun m v => put m v v) l empty_map.
+
+Definition Ex(p: Demos.Prog): example :=
+  let '(name, (inputVarList, outputVarList, src)) := p in
+  let inputVars: set var := of_list inputVarList in
+  let outputVars := of_list outputVarList in
+  let flattened := flatten src in
+  let regallocAnnotated := regalloc var var func
+         Register0
+         riscvRegisters
+         (list_to_id_map inputVarList)
+         flattened
+         empty_set
+         (list_to_id_map outputVarList) in
+  let regallocChecked :=
+    match checker var var func (list_to_id_map inputVarList) regallocAnnotated with
+    | Some s => s
+    | None => FlatImp.SSkip
+    end in
+  let riscv_instructions := FlatToRiscv.compile_stmt Lw Sw regallocChecked in
+  let riscv_words := List.map (fun i => ZToWord 32 (encode i)) riscv_instructions in
+  let riscv_word8s := store_word_list riscv_words
+                                      (Utility.ZToReg 0)
+                                      (zero_mem ((Memory.Zlength riscv_instructions) * 4)) in
+  let riscv_bytes := List.map (fun w => Byte.of_Z (uwordToZ w)) riscv_word8s in
+  mk_example
+    name
+    inputVars
+    outputVars
+    src
+    flattened
+    regallocAnnotated
+    regallocChecked
+    riscv_instructions
+    riscv_bytes.
+
+Time Definition allCompilationResults: list example :=
+  Eval cbv in (List.map Ex Demos.allProgs).
+
+Set Printing Width 100.
+Print allCompilationResults.
