compiler/src/examples/TestExprImp.v
@@ -49,6 +49,7 @@ Definition annoying_eq: DecidableEq
   (list varname * list varname * cmd). Admitted.
 Existing Instance annoying_eq.
 
+
 Definition run_isRight(x y z: Z): option word :=
   let final := eval_cmd empty_map 10 empty_map no_mem (isRight x y z) in
   match final with
